minuska/theories/spec_interpreter.v
@@ -1,0 +1,91 @@
+From Minuska Require Import
+    prelude
+    spec_syntax
+    spec_semantics
+    varsof
+    syntax_properties
+.
+
+
+Definition RewritingRule_wf1
+    {Σ : StaticModel}
+    (r : RewritingRule)
+    : Prop
+:= 
+    let vs1 : gset variable := vars_of (fr_scs r) in
+    let vs2 : gset variable := vars_of (fr_from r) in
+    (vs1 ⊆ vs2)
+.
+
+(*
+    This is known as 'weakly well-defined rule'
+    in the literature.
+*)
+Definition RewritingRule_wf2
+    {Σ : StaticModel}
+    (r : RewritingRule)
+    : Prop
+:= 
+    forall (g : GroundTerm) (ρ : Valuation),
+        satisfies ρ g (fr_from r) ->
+        satisfies ρ () (fr_scs r) ->
+        exists (g' : GroundTerm),
+            satisfies ρ g' (fr_to r)
+.
+
+Definition RewritingRule_wf
+    {Σ : StaticModel}
+    (r : RewritingRule)
+    : Prop
+:=
+    RewritingRule_wf1 r /\ RewritingRule_wf2 r
+.
+
+Definition RewritingTheory_wf
+    {Σ : StaticModel}
+    (Γ : RewritingTheory)
+    : Prop
+:=
+    Forall RewritingRule_wf Γ
+.
+
+Definition rewriting_relation_flat
+    {Σ : StaticModel}
+    (Γ : list RewritingRule)
+    : relation GroundTerm
+    := fun from to =>
+        exists r, r ∈ Γ /\ flattened_rewrites_to r from to
+.
+
+Definition not_stuck_flat
+    {Σ : StaticModel}
+    (Γ : list RewritingRule)
+    (e : GroundTerm) : Prop
+:= exists e', rewriting_relation_flat Γ e e'.
+
+Definition flat_stuck
+    {Σ : StaticModel}
+    (Γ : list RewritingRule)
+    (e : GroundTerm) : Prop
+:= not (not_stuck_flat Γ e).
+
+
+Definition FlatInterpreter
+    {Σ : StaticModel}
+    (Γ : list RewritingRule)
+    : Type
+    := GroundTerm -> option GroundTerm
+.
+
+Definition FlatInterpreter_sound
+    {Σ : StaticModel}
+    (Γ : list RewritingRule)
+    (wfΓ : RewritingTheory_wf Γ)
+    (interpreter : FlatInterpreter Γ)
+    : Prop
+    := (forall e,
+        flat_stuck Γ e -> interpreter e = None)
+    /\ (forall e,
+        not_stuck_flat Γ e ->
+        exists e', interpreter e = Some e')
+.
