minuska/theories/varsof.v
@@ -1,0 +1,152 @@
+From Minuska Require Import
+    prelude
+    spec_syntax
+.
+
+Fixpoint vars_of_Expression
+    {Σ : StaticModel}
+    (t : Expression)
+    : gset variable :=
+match t with
+| ft_element _ => ∅
+| ft_variable x => {[x]}
+| ft_nullary _ => ∅
+| ft_unary _ t' => vars_of_Expression t'
+| ft_binary _ t1 t2 => vars_of_Expression t1 ∪ vars_of_Expression t2
+| ft_ternary _ t1 t2 t3 => vars_of_Expression t1 ∪ vars_of_Expression t2 ∪ vars_of_Expression t3
+end.
+
+#[export]
+Instance VarsOf_Expression
+    {Σ : StaticModel}
+    : VarsOf Expression variable
+:= {|
+    vars_of := vars_of_Expression ; 
+|}.
+
+
+Definition vars_of_AP
+    {Σ : StaticModel}
+    (ap : AtomicProposition)
+    : gset variable :=
+match ap with
+| apeq e1 e2 => vars_of e1 ∪ vars_of e2
+end.
+
+#[export]
+Instance VarsOf_AP
+    {Σ : StaticModel}
+    : VarsOf AtomicProposition variable
+:= {|
+    vars_of := vars_of_AP ; 
+|}.
+
+Fixpoint vars_of_aosB
+    {Σ : StaticModel}
+    {B var : Type}
+    {_varED : EqDecision var}
+    {_varCnt : Countable var}
+    {_VB: VarsOf B var}
+    (o : AppliedOperator' symbol B)
+    : gset var :=
+match o with
+| ao_operator _ => ∅
+| ao_app_operand o' b => vars_of b ∪ vars_of_aosB o'
+| ao_app_ao o1 o2 => vars_of_aosB o1 ∪ vars_of_aosB o2
+end.
+
+#[export]
+Instance VarsOf_aosB
+    {Σ : StaticModel}
+    {B var : Type}
+    {_varED : EqDecision var}
+    {_varCnt : Countable var}
+    {_VB: VarsOf B var}
+    : VarsOf (AppliedOperator' symbol B) var
+:= {|
+    vars_of := vars_of_aosB ; 
+|}.
+
+Definition vars_of_BoV
+    {Σ : StaticModel}
+    (bov : BuiltinOrVar)
+    : gset variable
+:=
+match bov with
+| bov_variable x => {[x]}
+| bov_builtin _ => ∅
+end.
+
+#[export]
+Instance VarsOf_BoV
+    {Σ : StaticModel}
+    : VarsOf BuiltinOrVar variable
+:= {|
+    vars_of := vars_of_BoV ; 
+|}.
+
+Definition vars_of_OpenTerm
+    {Σ : StaticModel}
+    (φ : OpenTerm)
+    : gset variable :=
+match φ with
+| aoo_app o => vars_of o
+| aoo_operand bov => vars_of bov
+end.
+
+#[export]
+Instance VarsOf_OpenTerm 
+    {Σ : StaticModel}
+    : VarsOf OpenTerm variable
+:= {|
+    vars_of := vars_of_OpenTerm ; 
+|}.
+
+Definition vars_of_SideCondition
+    {Σ : StaticModel}
+    (c : SideCondition)
+    : gset variable :=
+match c with
+| sc_constraint c' => vars_of c'
+end.
+
+#[export]
+Instance VarsOf_SideCondition
+    {Σ : StaticModel}
+    : VarsOf SideCondition variable
+:= {|
+    vars_of := vars_of_SideCondition ; 
+|}.
+
+#[export]
+Program Instance VarsOf_list_SideCondition
+    {Σ : StaticModel}
+    : VarsOf (list SideCondition) variable
+:= {|
+    vars_of := fun scs => ⋃ (vars_of <$> scs)
+|}.
+
+Definition vars_of_AppliedOperatorOr'B
+    {Σ : StaticModel}
+    {B var : Type}
+    {_EDv : EqDecision var}
+    {_Cv : Countable var}
+    {_VB : VarsOf B var}
+    (φ : AppliedOperatorOr' symbol B)
+    : gset var :=
+match φ with
+| aoo_app aop => vars_of aop
+| aoo_operand otwsc => vars_of otwsc
+end.
+
+#[export]
+Instance VarsOf_AppliedOperatorOr'
+    {Σ : StaticModel}
+    {B var : Type}
+    {_EDv : EqDecision var}
+    {_Cv : Countable var}
+    {_VB : VarsOf B var}
+    : VarsOf (AppliedOperatorOr' symbol B) var
+:= {|
+    vars_of := vars_of_AppliedOperatorOr'B ; 
+|}.
